

# Homework Submission

## CMDA 3605 Mathematical Modeling: Methods and Tools I

---

### Virginia Tech Honor Code Pledge:

*"I have neither given nor received unauthorized assistance on this assignment."*

### Solution to Exercise 1

(a)

$$x(k+1) = f(x(k)) = Ax(k) + b$$

Taking the Jacobian of the evolution function  $f(x)$  yields:

$$J_f(x) = A$$

This is because taking the partial derivative of the entire function simply leaves  $A$  since  $b$  is just a constant.

(b) In order to show that the  $\det(J_g(r, \theta))$  is equal to  $r$ , compute the Jacobian given that the first column is the partial derivative with respect to  $r$  and the second column is the partial derivative with respect to  $\theta$ :

$$(J_g(r, \theta)) = \begin{bmatrix} \cos \theta & -r \sin \theta \\ \sin \theta & r \cos \theta \end{bmatrix}$$

Now compute the determinant ( $\det(J_g(r, \theta))$ ) of the Jacobian:

$$\begin{aligned} \det(J_g(r, \theta)) &= \begin{vmatrix} \cos \theta & -r \sin \theta \\ \sin \theta & r \cos \theta \end{vmatrix} \\ &= (\cos \theta)(r \cos \theta) + r \sin^2 \theta \\ &= r \cos^2 \theta + r \sin^2 \theta \\ &= r(\cos^2 \theta + \sin^2 \theta) \\ &= r(1) \end{aligned}$$

Therefore,  $\det(J_g(r, \theta)) = r$

## Solution to Exercise 2

Part (a)

Considering the nonlinear discrete dynamical system:

$$x(k+1) = ax(k)e^{-rx(k)}$$

Where  $a = e$  and  $r = 1$ . Then:

$$f(x) = exe^{-x} = e^{1-x}x$$

Before writing the linearization, we will need  $f'(x)$

$$f'(x) = -e^{1-x}x + e^{1-x}$$

Now looking at the linearization of the first steady state,  $\hat{x}_1 = 0$ .

$$u(k+1) = f'(\hat{x}_1)u(k)$$

where  $u(k)$  is  $(x(k) - \hat{x}_1)$ .

Now to determine the stability of  $\hat{x}_1$  we look at  $f'(\hat{x}_1)$

$$f'(\hat{x}_1) = -e^{1-0}(0) + e^1 \approx 2.7$$

Since  $|f'(\hat{x}_1)| > 1$  the steady state  $\hat{x}_1 = 0$  is an unstable steady state and we expect  $x(k)$  to drift away from  $\hat{x}_1$  for  $x_0 \neq \hat{x}_1$

Now looking at the linearization of the second steady state,  $\hat{x}_2 = 1$ .

$$u(k+1) = f'(\hat{x}_2)u(k)$$

where  $u(k)$  is  $(x(k) - \hat{x}_2)$ .

Now to determine the stability of  $\hat{x}_2$  we look at  $f'(\hat{x}_2)$

$$f'(\hat{x}_2) = -e^{1-1}(1) + e^{1-1} = -1 + 1 = 0$$

Since  $|f'(\hat{x}_2)| < 1$  the steady state  $\hat{x}_2 = 1$  is an asymptotically stable and we expect  $x(k)$  to approach  $\hat{x}_2$  for  $\|x_0 - \hat{x}_2\|$  small enough.

## Solution to Exercise 2 cont.

Part b

Considering the nonlinear dynamical system

$$f(x(k)) = \begin{bmatrix} x_1(k+1) \\ x_2(k+1) \end{bmatrix} = \begin{bmatrix} \frac{ax_1(k)x_2(k)}{1+x_1(k)} \\ \frac{bx_1(k)x_2(k)}{1+x_2(k)} \end{bmatrix}$$

where  $a = 1$  and  $b = 2$  Then:

$$f(x) = f\left(\begin{bmatrix} x_1 \\ x_2 \end{bmatrix}\right) = \begin{bmatrix} \frac{x_1x_2}{1+x_1} \\ \frac{2x_1x_2}{1+x_2} \end{bmatrix}$$

First we will need the Jacobian of F. Using the Quotient rule we get:

$$J(x) = \begin{bmatrix} \frac{x_2(1+x_1) - (x_1x_2)}{(1+x_1)^2} & \frac{x_1}{1+x_1} \\ \frac{2x_2}{1+x_2} & \frac{2x_1(1+x_2) - 2x_1x_2(1)}{(1+x_2)^2} \end{bmatrix}$$

simplified:

$$J(x) = \begin{bmatrix} \frac{x_2}{(1+x_1)^2} & \frac{x_1}{1+x_1} \\ \frac{2x_2}{1+x_2} & \frac{2x_1}{(1+x_2)^2} \end{bmatrix}$$

Now looking at the linearization of the first steady state,  $\hat{x}_1 = \begin{bmatrix} 0 \\ 0 \end{bmatrix}$ :

$$u(k+1) = J(\hat{x}_1)u(k)$$

Now to determine the stability of  $\hat{x}_1$  we look at  $J(\hat{x}_1)$

$$J\left(\begin{bmatrix} 0 \\ 0 \end{bmatrix}\right) = \begin{bmatrix} 0 & 0 \\ 0 & 0 \end{bmatrix}$$

Since  $S(J(\hat{x}_1)) = 0 < 1$  the steady state  $\begin{bmatrix} 0 \\ 0 \end{bmatrix}$  is an asymptotically stable steady state and we expect  $x(k)$  to approach  $\hat{x}_1$  for  $\|x_0 - \hat{x}_2\|$  small enough.

### Solution to Exercise 2 cont.

Now looking at the linearization of the second steady state,  $\hat{x}_2 = \begin{bmatrix} 2 \\ 3 \end{bmatrix}$ :

$$u(k+1) = J(\hat{x}_2)u(k)$$

Now to determine the stability of  $\hat{x}_2$  we look at  $J(\hat{x}_2)$

$$J\left(\begin{bmatrix} 3 \\ 3 \end{bmatrix}\right) = \begin{bmatrix} 3/9 & 2/3 \\ 6/4 & 4/16 \end{bmatrix}$$

Then we must find the eigenvalues to determine the spectral radius of the Jacobian at steady state two:

$$(1/3 - \lambda)(1/4 - \lambda) - 1 = \lambda^2 - 7/12\lambda - 11/12$$

Using the Pq formula to find roots of characteristic polynomial:

$$x_1 = 7/24 - \sqrt{(-7/14)^2 + 11/12}$$

$$= 7/24 - 1.0086767912 = -0.7092$$

$$x_2 = 7/24 + 1.0086767912 = 1.292534$$

So the eigenvalues of  $J(\hat{x}_2)$  are  $\lambda_1 = -0.7092$  and  $\lambda_2 = 1.2925$

Since  $S(J(\hat{x}_2)) = 1.2925 > 1$  the steady state  $\begin{bmatrix} 2 \\ 3 \end{bmatrix}$  is an unstable steady state and we expect  $x(k)$  to drift away from  $\hat{x}_2$  for  $x_0 \neq \hat{x}_2$

### Solution to Exercise 3

$$x(k+1) = f(x(k)) = x(k) - \frac{g(x(k))}{g'(x(k))}$$

The above equation can be written as:

$$f(\hat{x}) = \hat{x} - \frac{g(\hat{x})}{g'(\hat{x})}$$

Now compute the derivative, and utilize the quotient rule on the second term:

$$\begin{aligned} f'(x) &= 1 - \frac{d}{dx} \left( \frac{g(x)}{g'(x)} \right) \\ &= 1 - \frac{g'(x)g'(x) - g''(x)g(x)}{(g'(x))^2} \\ &= 1 - \frac{g'(x)^2 - g''(x)g(x)}{(g'(x))^2} \\ &= \frac{g(x)g''(x)}{(g''(x))^2} \end{aligned}$$

Now evaluating the equation at  $\hat{x}$ , given that  $g(\hat{x}) = 0$ , we can substitute this back into the above equation:

$$\begin{aligned} &= \frac{g(\hat{x})g''(\hat{x})}{(g''(\hat{x}))^2} \\ &= \frac{(0)g''(\hat{x})}{(g''(\hat{x}))^2} \\ &= 0 \end{aligned}$$

Since  $|f'(\hat{x})| = 0 < 1$ , we can conclude that  $\hat{x}$  is locally asymptotically stable and indicates that Newton's Method is locally convergent.

## Solution to Exercise 4

(a)

```
function [xr, res] = newtonmethod(g, J, x0, maxiter, tol)
x = x0;
res = zeros(maxiter, 1);

for k = 1:maxiter
    gx = g(x);

    res(k) = norm(gx, 2);
    fprintf('Iter %d: residual = %.3e\n', k, res(k));

    if res(k) < tol
        res = res(1:k);
        xr = x;
        return;
    endif

    d = -J(x) \ gx;

    x = x + d;
end
xr = x;
res = res(1:maxiter);
end
```

(b) Using the above Newton's method code with the function:

$$g(x) = \begin{bmatrix} x_1^2 + x_1 x_2^3 - 9 \\ 3x_1^2 x_2 - x_2^3 - 4 \end{bmatrix}$$

where

$$x = \begin{bmatrix} x_1 \\ x_2 \end{bmatrix}$$

, the root  $\hat{x}$  is equal to:

```
x hat =
1.3364
1.7542
```

(c) Using the initial value:

$$x_{0,1} = \begin{bmatrix} -3 \\ -3 \end{bmatrix}$$

### Solution to Exercise 4 cont.

The root  $\hat{x}$  is equal to:

```
Iter 1: residual = 9.962e+01
Iter 2: residual = 2.807e+01
Iter 3: residual = 6.618e+00
Iter 4: residual = 8.152e-01
Iter 5: residual = 1.180e-02
Iter 6: residual = 3.596e-06
Iter 7: residual = 2.251e-13
x hat =
-0.9013
-2.0866
```

Using the next initial value:

$$x_{0,2} = \begin{bmatrix} -3 \\ 3 \end{bmatrix}$$

The root  $\hat{x}$  is equal to:

```
Iter 1: residual = 9.519e+01
Iter 2: residual = 3.117e+01
Iter 3: residual = 1.190e+01
Iter 4: residual = 7.629e+00
Iter 5: residual = 2.735e+01
Iter 6: residual = 7.035e+00
Iter 7: residual = 7.848e-01
Iter 8: residual = 4.407e-03
Iter 9: residual = 4.195e-07
Iter 10: residual = 0.000e+00
x hat =
-3.0016
0.1481
```

Lastly, using the third initial value:

$$x_{0,2} = \begin{bmatrix} 4 \\ 0 \end{bmatrix}$$

### Solution to Exercise 4 cont.

The root  $\hat{x}$  is equal to:

```
Iter 1: residual = 8.062e+00
Iter 2: residual = 1.738e+00
Iter 3: residual = 1.343e-01
Iter 4: residual = 3.150e-04
Iter 5: residual = 1.826e-09
Iter 6: residual = 2.220e-15
x hat =
    2.9984
    0.1484
```

**Observations:** For the first initial value  $x_{0,1} = \begin{bmatrix} -3 \\ -3 \end{bmatrix}$ , the method converged after 7 iterations according to the output of the code. The residuals appear to converge rapidly as the first iteration starts at  $\approx 9.96 * 10^1$  and ends at the last iteration with a value much lower of  $\approx 2.25 * 10^{-13}$ . For the initial value  $x_{0,1} = \begin{bmatrix} -3 \\ -3 \end{bmatrix}$ , newton's method converged to the root  $\hat{x} = \begin{bmatrix} -0.9013 \\ -2.0866 \end{bmatrix}$ .

For the second initial value  $x_{0,2} = \begin{bmatrix} -3 \\ 3 \end{bmatrix}$ , the residuals decreased rapidly all the way to 0 after 10 iterations. Since the residuals approached 0, this indicates that the method was able to successfully calculate a solution where  $g(x) = 0$ . For the initial value  $x_{0,1} = \begin{bmatrix} -3 \\ 3 \end{bmatrix}$ , newton's method converged to the root  $\hat{x} = \begin{bmatrix} -3.0016 \\ 0.1481 \end{bmatrix}$ .

For the last initial value  $x_{0,3} = \begin{bmatrix} 4 \\ 0 \end{bmatrix}$ , relative to the other two initial values the residuals decreased more rapidly as it only experienced 6 iterations. This indicates that the initial guess was close to the true root, since the iterations converged faster than the other initial values. For the initial value  $x_{0,3} = \begin{bmatrix} 4 \\ 0 \end{bmatrix}$ , newton's method converged to the root  $\hat{x} = \begin{bmatrix} 2.9984 \\ 0.1484 \end{bmatrix}$ .



## Solution to Exercise 5

Part a

Define the nonlinear function

$$f_1(x) = x - g(x) = x - x^3 - 4x^2 + 10$$

with

$$g(x) = x^3 + 4x^2 - 10$$

To verify that  $\hat{x}$  is a fixed point of  $f_1$ , then  $g(\hat{x}) = 0$  we need, that if  $\hat{x}$  is a fixed point of  $f_1$ , then  $f_1(\hat{x}) = \hat{x}$ .

Then

$$f_1(\hat{x}) = \hat{x} - g(\hat{x}) = \hat{x}$$

Therefore,  $g(\hat{x}) = 0$  must be true.

After running the fixed point iteration, this is output vector shows F1 as  $x(k+1) = f_1(x(k))$ .  $x(0) = 1.5$

```
Columns 1 through 11:
    1.5000   -0.8750    6.7324  -469.7200  102754555.1874  -1084933870531746352594944.0000  127
378074254579861314550183250535909418315265493330570988486656.0000  -208271290858102499745717
03354901622173836675970995448130575801767295649567106614767785401768557086338743510717499427
374341691407014825950224181484247938321688218219358704615541966960319844958863360.0000
aN      NaN

Columns 12 through 22:
      NaN      NaN      NaN      NaN      NaN      NaN      NaN      NaN      NaN      NaN

Columns 23 through 33:
      NaN      NaN      NaN      NaN      NaN      NaN      NaN      NaN      NaN      NaN
```

This shows that the iteration is not converging, but is diverging. Now consider the linearization of  $f_1$  on  $\hat{x} \approx 1.365230013414097$

$$u(k+1) = f'_1(\hat{x})u(k)$$

$$u(k) = (f_1(k) - \hat{x})$$

and

$$f'_1(x) = 1 - 3x^2 - 8x$$

now check the stability

$$f'_1(\hat{x}) = 1 - 3(1.36523)^2 - 8(1.36523) \approx -15.513$$

Since  $|f'_1(\hat{x})| > 1$  the linearization of  $f_1$  on the given root is unstable, and the iteration does not converge with  $x(0) = 1.5$

## Solution to Exercise 5 cont.

Part b

After running the fixed point iteration, this is output vector shows F2 as  $x(k+1) = f_2(x(k))$ .  
 $x(0) = 1.5$

```
Columns 1 through 11:
    1.5000    1.2870    1.4025    1.3455    1.3752    1.3601    1.3678    1.3639    1.3659    1.3649    1.3654
Columns 12 through 22:
    1.3651    1.3653    1.3652    1.3652    1.3652    1.3652    1.3652    1.3652    1.3652    1.3652    1.3652
Columns 23 through 33:
    1.3652    1.3652    1.3652    1.3652    1.3652    1.3652    1.3652    1.3652    1.3652    1.3652    1.3652
Columns 34 through 44:
    1.3652    1.3652    1.3652    1.3652    1.3652    1.3652    1.3652    1.3652    1.3652    1.3652    1.3652
Columns 45 through 51:
    1.3652    1.3652    1.3652    1.3652    1.3652    1.3652    1.3652
>> |
```

This shows that the iteration does converge to the desired root.  
 Now consider the linearization of  $f_2$  on  $\hat{x} \approx 1.365230013414097$

$$u(k+1) = f'_2(\hat{x})u(k)$$

$$u(k) = (f_2(k) - \hat{x})$$

Solving for  $f'_2$

$$f_2(x) = \frac{1}{2}(10 - x^3)^{\frac{1}{2}}$$

let  $z(k) = 10 - x^3$   
 and  $z'(k) = -3x^2$

$$f_2(x) = \frac{1}{2}u(k)^{\frac{1}{2}}$$

$$f'_2(x) = \frac{1}{2} \times \frac{1}{2}u(k)^{-\frac{1}{2}}u'(k)$$

$$f'_2(x) = (1/2)(1/2)(10 - x^3)^{-1/2}(-3x)^2$$

$$f'_2(x) = -\frac{3x^2}{4(10 - x^3)^{1/2}}$$

now check the stability

$$f'_2(\hat{x}) = -\frac{3(1.3652)^2}{4(10 - (1.3652)^3)^{1/2}} \approx -0.51196125503$$

Since  $|f'_2(\hat{x})| < 1$  the linearization of the fixed point iteration on  $f_2$  is asymptotically stable.  
 $u(k) \rightarrow 0$  and  $f_2(k) \rightarrow \hat{x}$

## Solution to Exercise 5 cont.

Part c

After running the fixed point iteration, this is output vector shows F3 as  $x(k+1) = f_3(x(k))$ .  
 $x(0) = 1.5$

```
Columns 1 through 11:
    1.5000    1.3733    1.3653    1.3652    1.3652    1.3652    1.3652    1.3652    1.3652    1.3652    1.3652
Columns 12 through 22:
    1.3652    1.3652    1.3652    1.3652    1.3652    1.3652    1.3652    1.3652    1.3652    1.3652    1.3652
Columns 23 through 33:
    1.3652    1.3652    1.3652    1.3652    1.3652    1.3652    1.3652    1.3652    1.3652    1.3652    1.3652
Columns 34 through 44:
    1.3652    1.3652    1.3652    1.3652    1.3652    1.3652    1.3652    1.3652    1.3652    1.3652    1.3652
Columns 45 through 51:
    1.3652    1.3652    1.3652    1.3652    1.3652    1.3652    1.3652
```

This shows that the iteration does converge to the desired root even faster than the previous iteration.

Now consider the linearization of  $f_3$  on  $\hat{x} \approx 1.365230013414097$

$$u(k+1) = f'_3(\hat{x})u(k)$$

$$u(k) = (f_3(k) - \hat{x})$$

Using the quotient rule we get:

$$f'_3(x) = 1 - \frac{(3x^2 + 8x)(3x^2 + 8x) - (x^3 + 4x^2 - 10)(6x + 8)}{(3x^2 + 8x)^2}$$

Now we check the stability

$$f'_3(x) = -0.0000294$$

Since  $|f'_3(\hat{x})| < 1$  the linearization is asymptotically stable.  $u(k) \rightarrow 0$  and  $f_2(k) \rightarrow \hat{x}$